system-f/Substitution.v
@@ -7,22 +7,121 @@ Require Export Arith.
 Open Scope t_scope.
 Open Scope list_scope.
 
-Reserved Notation " [ γ ! n ] M " (at level 5).
-Reserved Notation " [ K ↑ n ] M " (at level 5).
+Reserved Notation " [ A /// n ] B " (at level 5).
+Reserved Notation " [ A // n ] t " (at level 5).
+Reserved Notation " [ s \ n ] t " (at level 5).
+(* Oddly, I can’t seem to get it working with [ s / n ] *)
+Reserved Notation " [ γ ! n ] t " (at level 5).
 
-(* Substitution of index n for term K in M *)
-Fixpoint subt K n M :=
-  match M with
-    | #m => if (eq_nat_dec n m) then K else M
-    | λ A, M => λ A, [K ↑ S n]M
-    | M @ N => [K ↑ n]M @ [K ↑ n]N
-    | z => z
-    | s M => s [K ↑ n]M
-    | rec M M₀ M₁ => rec [K ↑ n]M [K ↑ n]M₀ [K ↑ S (S n)]M₁
-    | hd M => hd [K ↑ n]M
-    | tl M => tl [K ↑ n]M
-    | seed M M₀ M₁ => seed [K ↑ n]M [K ↑ S n]M₀ [K ↑ S n]M₁
-  end where " [ K ↑ n ] M " := (subt K n M) : t_scope.
+(* “bump k A” increments all except the first k free vars in A *)
+(* variants for type/term vars in types/terms *)
+
+Fixpoint ty_bump_ty (k:nat) (A:ty) :=
+  match A with
+    | ##n => if (lt_dec n k) then ##n else ##(S n)
+    | A arrows B => (ty_bump_ty k A) arrows (ty_bump_ty k B)
+    | allX, A => allX, (ty_bump_ty (S k) A)
+  end.
+
+Fixpoint ty_bump_tm (k:nat) (t:tm) :=
+  match t with
+    | #n => #n
+    | λx A, t0 => λx (ty_bump_ty k A), (ty_bump_tm k t0)
+    | t0 * t1 => (ty_bump_tm k t0) * (ty_bump_tm k t1)
+    | ΛX, t0 => ΛX, (ty_bump_tm (S k) t0)
+    | t0 @ A => (ty_bump_tm k t0) @ (ty_bump_ty k A)
+  end.
+
+Fixpoint tm_bump_tm (k:nat) (t:tm) :=
+  match t with
+    | #n => if (lt_dec n k) then #n else #(S n)
+    | λx A, t0 => λx A, (tm_bump_tm (S k) t0)
+    | t0 * t1 => (tm_bump_tm k t0) * (tm_bump_tm k t1)
+    | ΛX, t0 => ΛX, (tm_bump_tm k t0)
+    | t0 @ A => (tm_bump_tm k t0) @ A
+  end.
+
+(* To understand the “unbumping” in substitution, think about how the variables of A, B (resp. s, t) should match up after an inst-reduction (resp. β-reduction) under a binder. *)
+
+(* Substitution of type A for index n in B *)
+Fixpoint ty_sub_ty A n B :=
+  match B with
+    | ##k => if (eq_nat_dec k n) then A else
+             if (lt_dec k n) then ##k else ##(pred k)
+    | B0 arrows B1 => ([A /// n] B0) arrows ([A /// n] B1)
+    | allX, B0 => allX, [ty_bump_ty 0 A /// S n]B0
+  end
+where " [ A /// n ] B " := (ty_sub_ty A n B) : t_scope.
+
+(* Substitution of type A for index n in t *)
+Fixpoint ty_sub_tm A n t :=
+  match t with
+    | #k => #k
+    | λx B, t0 => λx ([A /// n] B), [A // n] t0
+    | t0 * t1 => [A//n]t0 * [A//n]t1
+    | ΛX, t0 => ΛX, [ty_bump_ty 0 A // S n] t0
+    | t0 @ B => ([A // n] t0) @ ([A /// n] B)
+  end
+where " [ A // n ] t " := (ty_sub_tm A n t) : t_scope.
+
+
+(* Substitution of term s for index n in t *)
+Fixpoint tm_sub_tm s n t :=
+  match t with
+    | #k => if (eq_nat_dec k n) then s else
+             if (lt_dec k n) then #k else #(pred k)
+    | λx A, t0 => λx A, tm_sub_tm (tm_bump_tm 0 s) (S n) t0
+    | t0 * t1 => (tm_sub_tm s n t0) * (tm_sub_tm s n t1)
+    | ΛX, t0 => ΛX, (tm_sub_tm (ty_bump_tm 0 s) n t0)
+    | t0 @ B => ([s \ n] t0) @ B
+  end
+where " [ s \ n ] t " := (tm_sub_tm s n t) : t_scope.
+
+(* Substitution for the list γ, starting from index n in M *)
+(* Not — *not* simultaneous; done in order. *)
+Fixpoint list_sub_tm (γ : list tm) (n : nat) (t : tm) :=
+  match γ with
+    | nil => t
+    | s :: γ => [γ!n][s \ n]t
+  end
+where " [ γ ! n ] t " := (list_sub_tm γ n t) : t_scope.
+
+Lemma list_sub_lam γ : forall n A t,
+  [γ!n](λx A, t) = (λx A, [(List.map (tm_bump_tm 0) γ)!(S n)]t).
+Proof.
+  induction γ as [ | s γ' IH]; intros.
+  (* Case γ = nil *) auto.
+  (* Case γ = s :: γ' *) simpl. apply IH.
+Qed.
+
+(*
+Lemma list_sub_commute : forall γ t w,
+  ([w\0] [List.map (tm_bump_tm 0) γ ! 1] t)
+  = [ ([γ!0]w :: γ) ! 0 ] t.
+Proof.
+  induction γ as [ | s γ' IHγ'].
+  (* case γ = nil *)  reflexivity.
+  (* case γ = s :: γ' *) induction t as [ n | A t IH | t0 IH0 t1 IH1 | t IH | t IH A]; simpl.
+*)
+
+
+(*  For some reason, the parser doesn’t like the notations in the following; it also doesn’t work with [ s % n] t; but it does work with [ s %% n ] t!
+
+Reserved Notation " [ s / n ] t " (at level 5).
+
+Fixpoint tm_sub_tm s n t :=
+  match t with
+    | #k => if (eq_nat_dec k n) then s else #k
+    | λx A, t0 => λx A, [ (tmbumptm 0 s) / (S n] t0
+    | t0 * t1 => [ s / n ] t0 * [s / n]t1
+    | ΛX, t0 => ΛX, [tybumptm 0 s / n] t0
+    | t0 @ B => ([s / n] t0) @ B
+  end
+where " [ s / n ] t " := (tm_sub_tm s n t) : t_scope.
+*)
+
+
+(* From here on is finrod’s original version:
 
 (* Substitution for the list γ, starting from index n in M *)
 Fixpoint sub (γ : list te) (n : nat) (M : te) :=
@@ -76,7 +175,7 @@ Proof.
   rewrite IHγ; simpl; reflexivity.
 Qed.
 Lemma sub_rec : forall γ n M M₀ M₁,
-  ([γ ! n](rec M M₀ M₁)) = rec [γ ! n]M [γ ! n]M₀ [γ ! S (S n)]M₁.
+  ([γ ! n](rec M M₀ M₁)) = rec [γ ! n]M [γ ! n]M₀ [γ ! S (S n]M₁.
 Proof.
   induction γ; intros; simpl in *; [reflexivity |].
   rewrite IHγ; simpl; reflexivity.
@@ -99,6 +198,8 @@ Proof.
   induction γ; intros; simpl in *; [reflexivity |].
   rewrite IHγ; simpl; reflexivity.
 Qed.
+
+*)
 
 Close Scope list_scope.
 Close Scope t_scope.
