system-f/Syntax.v
@@ -1,30 +1,39 @@
-(** This file defines the syntax of the System T extended with stream types. *)
+(** This file defines the syntax of System F.  Based on Filip’s development of System T. (github.com/finrod) *)
 
+ 
 (* Types *)
 Inductive ty :=
-| tnat : ty
-| tarrow : ty -> ty -> ty
-| stream : ty -> ty.
+| tvar    : nat -> ty
+| tarrow  : ty -> ty -> ty
+| tforall : ty -> ty.
 
-Notation " A '→' B " := (tarrow A B) (at level 30, right associativity) : t_scope.
-Notation " 'ω' " := tnat : t_scope.
+Notation " ## n " := (tvar n) (at level 20) : t_scope.
+Notation " A 'arrows' B " := (tarrow A B) (at level 30, right associativity) : t_scope.
+Notation "'allX' , A " := (tforall A) (at level 50) : t_scope.
 Open Scope t_scope.
 
 (* Terms *)
 (* The formalisation uses de Bruijn indices to deal with binders. *)
-Inductive te :=
-| var  : nat -> te
-| lam  : ty -> te -> te
-| appl : te -> te -> te
-| z    : te
-| s    : te -> te
-| rec  : te -> te -> te -> te
-| hd   : te -> te
-| tl   : te -> te
-| seed : te -> te -> te -> te.
+Inductive tm :=
+| var  : nat -> tm
+| lam  : ty -> tm -> tm
+| appl : tm -> tm -> tm
+| Lam  : tm -> tm
+| inst : tm -> ty -> tm.
 
-Notation "'λ' A , M " := (lam A M) (at level 50) : t_scope.
 Notation " # n " := (var n) (at level 20) : t_scope.
-Notation " M @ N " := (appl M N) (at level 40, left associativity) : t_scope.
+Notation "'λx' A , t " := (lam A t) (at level 50) : t_scope.
+Notation " t * s " := (appl t s) (at level 40, left associativity) : t_scope.
+Notation "'ΛX' , t" := (Lam t) (at level 50) : t_scope.
+Notation " t @ A " := (inst t A) (at level 40, left associativity) : t_scope.
+
+Fixpoint closed (n:nat) (t:tm) : Prop :=
+match t with 
+  | #k => k < n
+  | λx A, t' => closed (S n) t'
+  | s0 * s1 => closed n s0 /\ closed n s1
+  | ΛX, t' => closed n t'
+  | s @ A => closed n s
+end.
 
 Close Scope t_scope.
